Split TreeSync API, start TreeSync spec hierarchy

fstar/MLS.fst
@@ -2,7 +2,7 @@ module MLS
 
 open Comparse
 open MLS.Tree
-open MLS.TreeSync.Types
+open MLS.TreeSync.Level0.Types
 open MLS.Crypto
 open MLS.NetworkTypes
 open MLS.TreeSync.NetworkTypes
@@ -13,6 +13,7 @@ open MLS.TreeSyncTreeKEMBinder
 open MLS.TreeSync.Extensions
 open MLS.TreeDEM.KeyPackageRef
 open MLS.TreeKEM
+open MLS.TreeKEM.API.Types
 open MLS.TreeDEM.Message.Types
 open MLS.TreeDEM.Message.Content
 open MLS.TreeDEM.Message.Framing
@@ -35,7 +36,7 @@ let universal_sign_nonce =
 let group_id = bytes
 
 type state = {
-  treesync_state: MLS.TreeSync.Types.state_t bytes tkt;
+  treesync_state: MLS.TreeSync.API.Types.state_t bytes tkt;
   treekem_state: treekem_state bytes;
   leaf_index: nat;
   leaf_secret: bytes;
@@ -102,19 +103,19 @@ val process_proposal: nat -> state -> proposal bytes -> result state
 let process_proposal sender_id st p =
   match p with
   | Add key_package ->
-    tmp <-- MLS.TreeSync.add st.treesync_state key_package;
+    tmp <-- MLS.TreeSync.API.add st.treesync_state key_package;
     let (treesync_state, _) = tmp in
     assume (length #bytes key_package.tbs.leaf_node.data.content = hpke_public_key_length #bytes);
-    let (treekem_state, _) = MLS.TreeKEM.add st.treekem_state ({version = 0; public_key = key_package.tbs.leaf_node.data.content;}) in
+    let (treekem_state, _) = MLS.TreeKEM.API.add st.treekem_state ({version = 0; public_key = key_package.tbs.leaf_node.data.content;}) in
     return ({ st with treesync_state; treekem_state })
   | Update leaf_package ->
     if not (sender_id < pow2 st.treesync_state.levels) then
       error "process_proposal: leaf_ind is greater than treesize"
     else (
-      let treesync_state = MLS.TreeSync.update st.treesync_state leaf_package sender_id in
+      let treesync_state = MLS.TreeSync.API.update st.treesync_state leaf_package sender_id in
       assume (length #bytes leaf_package.data.content = hpke_public_key_length #bytes);
       assume(st.treesync_state.levels == st.treekem_state.levels);
-      let treekem_state = MLS.TreeKEM.update st.treekem_state ({version = 0; public_key = leaf_package.data.content}) sender_id in
+      let treekem_state = MLS.TreeKEM.API.update st.treekem_state ({version = 0; public_key = leaf_package.data.content}) sender_id in
       return ({ st with treesync_state; treekem_state })
     )
   | Remove leaf_index ->
@@ -122,8 +123,8 @@ let process_proposal sender_id st p =
       error "process_proposal: leaf_index too big"
     else (
       assume(st.treesync_state.levels == st.treekem_state.levels);
-      let treesync_state = MLS.TreeSync.remove st.treesync_state leaf_index in
-      let treekem_state = MLS.TreeKEM.remove st.treekem_state leaf_index in
+      let treesync_state = MLS.TreeSync.API.remove st.treesync_state leaf_index in
+      let treekem_state = MLS.TreeKEM.API.remove st.treekem_state leaf_index in
       return ({ st with treesync_state; treekem_state })
     )
   | _ -> error "process_proposal: not implemented"
@@ -175,12 +176,12 @@ let process_commit state message message_auth =
         uncompressed_path <-- uncompress_update_path sender_id state.treesync_state.tree path;
         let treesync_path = update_path_to_treesync uncompressed_path in
         treekem_path <-- update_path_to_treekem group_context_bytes uncompressed_path;
-        treesync_path_valid <-- MLS.TreeSync.external_path_is_valid state.treesync_state.tree treesync_path state.treesync_state.group_id;
+        treesync_path_valid <-- MLS.TreeSync.Level0.external_path_is_valid state.treesync_state.tree treesync_path state.treesync_state.group_id;
         if not treesync_path_valid then
           error "process_commit: invalid update path"
         else (
-          treesync_state <-- MLS.TreeSync.commit state.treesync_state treesync_path;
-          let treekem_state = MLS.TreeKEM.commit state.treekem_state treekem_path in
+          treesync_state <-- MLS.TreeSync.API.commit state.treesync_state treesync_path;
+          let treekem_state = MLS.TreeKEM.API.commit state.treekem_state treekem_path in
           return ({ state with treesync_state; treekem_state;})
         )
       )
@@ -318,7 +319,7 @@ let fresh_key_package e cred private_sign_key =
   hash <-- hash_leaf_package key_package.tbs.leaf_node;
   return (key_package_bytes, hash, leaf_secret)
 
-let current_epoch s = s.treesync_state.MLS.TreeSync.Types.version
+let current_epoch s = s.treesync_state.MLS.TreeSync.API.Types.version
 
 #push-options "--fuel 2 --z3rlimit 50"
 let create e cred private_sign_key group_id =
@@ -326,7 +327,7 @@ let create e cred private_sign_key group_id =
   let fresh, e = tmp in
   tmp <-- fresh_key_package_internal fresh cred private_sign_key;
   let key_package, leaf_secret = tmp in
-  let treesync_state = MLS.TreeSync.create group_id key_package.tbs.leaf_node in
+  let treesync_state = MLS.TreeSync.API.create group_id key_package.tbs.leaf_node in
   treekem <-- treesync_to_treekem treesync_state.tree;
   let treekem_state: treekem_state bytes = { levels = 0; tree = treekem } in
   // 10. In principle, the above process could be streamlined by having the
@@ -497,7 +498,7 @@ let generate_update_path st e proposals =
       };
     }) in
     update_path_ext_sync <-- treekem_to_treesync my_new_leaf_package update_path_kem;
-    update_path_sync <-- MLS.TreeSync.external_path_to_valid_external_path st.treesync_state.tree update_path_ext_sync st.treesync_state.group_id st.sign_private_key sign_nonce;
+    update_path_sync <-- MLS.TreeSync.Level0.external_path_to_valid_external_path st.treesync_state.tree update_path_ext_sync st.treesync_state.group_id st.sign_private_key sign_nonce;
     uncompressed_update_path <-- mls_star_paths_to_update_path update_path_sync update_path_kem;
     update_path <-- compress_update_path uncompressed_update_path;
     let new_key_package_bytes = (ps_to_pse (ps_leaf_node_nt tkt)).serialize_exact update_path.leaf_node in
