fstar/MLS.TreeKEM.API.fst
@@ -1,0 +1,39 @@
+module MLS.TreeKEM.API
+
+open Comparse
+open MLS.Crypto
+open MLS.TreeCommon
+open MLS.TreeKEM.Types
+open MLS.TreeKEM
+open MLS.TreeKEM.API.Types
+
+val state_update_tree: #bytes:Type0 -> {|crypto_bytes bytes|} -> #l:nat -> treekem_state bytes -> treekem bytes l 0 -> treekem_state bytes
+let state_update_tree #bytes #bl #l st new_tree =
+  ({ st with
+    levels = l;
+    tree = new_tree;
+  })
+
+val add: #bytes:Type0 -> {|crypto_bytes bytes|} -> treekem_state bytes -> member_info bytes -> treekem_state bytes & nat
+let add #bytes #cb st kp =
+  match find_empty_leaf st.tree with
+  | Some i ->
+    (state_update_tree st (tree_add st.tree i kp), (i <: nat))
+  | None ->
+    let augmented_tree = add_one_level st.tree in
+    let i = Some?.v (find_empty_leaf augmented_tree) in
+    (state_update_tree st (tree_add augmented_tree i kp), (i <: nat))
+
+val update: #bytes:Type0 -> {|crypto_bytes bytes|} -> st:treekem_state bytes -> member_info bytes -> treekem_index st -> treekem_state bytes
+let update #bytes #cb st lp i =
+  state_update_tree st (tree_update st.tree i lp)
+
+val remove: #bytes:Type0 -> {|crypto_bytes bytes|} -> st:treekem_state bytes -> i:treekem_index st -> treekem_state bytes
+let remove #bytes #cb st i =
+  let blanked_tree = (tree_remove st.tree i) in
+  let (|_, reduced_tree|) = canonicalize_tree blanked_tree in
+  state_update_tree st reduced_tree
+
+val commit: #bytes:Type0 -> {|crypto_bytes bytes|} -> st:treekem_state bytes -> #li:treekem_index st -> pathkem bytes st.levels 0 li -> treekem_state bytes
+let commit #bytes #cb st #li p =
+  state_update_tree st (tree_apply_path st.tree p)
