fstar/MLS.TreeSync.API.Types.fst
@@ -1,0 +1,15 @@
+module MLS.TreeSync.API.Types
+
+open Comparse
+open MLS.TreeSync.NetworkTypes
+open MLS.TreeSync.Level0.Types
+
+(** TreeSync state and accessors *)
+type state_t (bytes:Type0) {|bytes_like bytes|} (tkt:treekem_types bytes) = {
+  group_id: bytes;
+  levels: nat;
+  tree: treesync bytes tkt levels 0;
+  version: nat;
+}
+
+type index_t (#bytes:Type0) {|bytes_like bytes|} (#tkt:treekem_types bytes) (st:state_t bytes tkt) = i:nat{i < pow2 st.levels}
