fstar/MLS.TreeSync.API.fst
@@ -1,0 +1,65 @@
+module MLS.TreeSync.API
+
+open Comparse
+open MLS.Crypto
+open MLS.TreeSync.NetworkTypes
+open MLS.Tree
+open MLS.TreeCommon
+open MLS.TreeSync.Level0.Types
+open MLS.TreeSync.Level0
+open MLS.TreeSync.API.Types
+open MLS.Result
+
+val create: #bytes:Type0 -> {|bytes_like bytes|} -> #tkt:treekem_types bytes -> gid:bytes -> leaf_node_nt bytes tkt -> state_t bytes tkt
+let create #bytes #bl gid lp =
+  {
+    group_id = gid;
+    levels = 0;
+    tree = create_tree lp;
+    version = 0;
+  }
+
+val state_update_tree: #bytes:Type0 -> {|bytes_like bytes|} -> #tkt:treekem_types bytes -> #l:nat -> state_t bytes tkt -> treesync bytes tkt l 0 -> state_t bytes tkt
+let state_update_tree #bytes #bl #tkt #l st new_tree =
+  ({ st with
+    levels = l;
+    version = st.version + 1;
+    tree = new_tree;
+  })
+
+val get_leaf_package_from_key_package: #bytes:Type0 -> {|crypto_bytes bytes|} -> #tkt:treekem_types bytes -> key_package_nt bytes tkt -> result (leaf_node_nt bytes tkt)
+let get_leaf_package_from_key_package #bytes #cb kp =
+  //TODO check signature
+  if not (kp.tbs.leaf_node.data.source = LNS_key_package ()) then
+    error "get_leaf_package_from_key_package: source is not add"
+  else (
+    return kp.tbs.leaf_node
+  )
+
+val add: #bytes:Type0 -> {|crypto_bytes bytes|} -> #tkt:treekem_types bytes -> state_t bytes tkt -> key_package_nt bytes tkt -> result (state_t bytes tkt & nat)
+let add #bytes #bl #tkt st kp =
+  lp <-- get_leaf_package_from_key_package kp;
+  match find_empty_leaf st.tree with
+  | Some i ->
+    new_tree <-- tree_add st.tree i lp;
+    return (state_update_tree st new_tree, (i <: nat))
+  | None ->
+    let augmented_tree = add_one_level st.tree in
+    let i = Some?.v (find_empty_leaf augmented_tree) in
+    new_tree <-- tree_add augmented_tree i lp;
+    return (state_update_tree st new_tree, (i <: nat))
+
+val update: #bytes:Type0 -> {|bytes_like bytes|} -> #tkt:treekem_types bytes -> st:state_t bytes tkt -> leaf_node_nt bytes tkt -> index_t st -> state_t bytes tkt
+let update #bytes #bl #tkt st lp i =
+  state_update_tree st (tree_update st.tree i lp)
+
+val remove: #bytes:Type0 -> {|bytes_like bytes|} -> #tkt:treekem_types bytes -> st:state_t bytes tkt -> i:index_t st -> state_t bytes tkt
+let remove #bytes #bl #tkt st i =
+  let blanked_tree = (tree_remove st.tree i) in
+  let (|_, reduced_tree|) = canonicalize_tree blanked_tree in
+  state_update_tree st reduced_tree
+
+val commit: #bytes:Type0 -> {|crypto_bytes bytes|} -> #tkt:treekem_types bytes -> st:state_t bytes tkt -> #li:index_t st -> external_pathsync bytes tkt st.levels 0 li -> result (state_t bytes tkt)
+let commit #bytes #cb #tkt st #li p =
+  new_tree <-- apply_external_path st.tree p;
+  return (state_update_tree st new_tree)
