fstar/MLS.TreeSync.Hash.fst
@@ -2,10 +2,10 @@ module MLS.TreeSync.Hash
 
 open Comparse
 open MLS.Tree
-open MLS.TreeSync.Types
 open MLS.Crypto
 open MLS.NetworkTypes
 open MLS.TreeSync.NetworkTypes
+open MLS.TreeSync.Level0.Types
 open MLS.Result
 
 #set-options "--fuel 1 --ifuel 1"
