fstar/MLS.TreeSync.Level0.Types.fst
@@ -1,0 +1,11 @@
+module MLS.TreeSync.Level0.Types
+
+open Comparse
+open MLS.Tree
+open MLS.TreeSync.NetworkTypes
+
+let treesync (bytes:Type0) {|bytes_like bytes|} (tkt:treekem_types bytes) =
+  tree (option (leaf_node_nt bytes tkt)) (option (parent_node_nt bytes tkt))
+
+let external_pathsync (bytes:Type0) {|bytes_like bytes|} (tkt:treekem_types bytes) =
+  path (leaf_node_nt bytes tkt) (option tkt.node_content)
